theories/lang/subst_map.v
@@ -48,6 +48,8 @@ Fixpoint subst_map (vs : gmap string val) (e : expr) : expr :=
       Load (subst_map vs e)
   | Store e1 e2 =>
       Store (subst_map vs e1) (subst_map vs e2)
+  | Replace e1 e2 =>
+      Replace (subst_map vs e1) (subst_map vs e2)
   end
 .
 
